Clase5.Listas.fst
@@ -11,12 +11,17 @@ let rec sum_int xs =
 (* Demuestre que sum_int "distribuye" sobre la concatenación de listas. *)
 let rec sum_append (l1 l2 : list int)
   : Lemma (sum_int (l1 @ l2) == sum_int l1 + sum_int l2)
-  = admit()
+  =
+  match l1 with
+  | [] -> ()
+  | x::xs -> (
+    sum_append xs l2
+  )
 
 (* Idem para length, definida en la librería de F*. *)
-let rec len_append (l1 l2 : list int)
+let len_append (l1 l2 : list int)
   : Lemma (length (l1 @ l2) == length l1 + length l2)
-  = admit()
+  = ()
 
 let rec snoc (xs : list int) (x : int) : list int =
   match xs with
@@ -32,14 +37,50 @@ let rec rev_int (xs : list int) : list int =
   | [] -> []
   | x::xs' -> snoc (rev_int xs') x
 
-let rev_append_int (xs ys : list int)
-  : Lemma (rev_int (xs @ ys) == rev_int ys @ rev_int xs)
-= admit()
+let rec snoc_append (xs ys : list int) (y : int) : Lemma (snoc (xs@ys) y == xs @ (snoc ys y)) =
+  match xs with
+  | [] -> ()
+  | x::xs' -> (
+    snoc_append xs' ys y
+  )
 
-let rev_rev (xs : list int)
+let rec rev_append_int (xs ys : list int)
+  : Lemma (rev_int (xs @ ys) == rev_int ys @ rev_int xs) =
+  match xs with
+  | [] -> ()
+  | x::xs' -> (
+    rev_append_int xs' ys;
+    snoc_append (rev_int ys) (rev_int xs') x
+  )
+
+let rec rev_aux (xs : list int) (x : int) : Lemma (rev_int (snoc xs x) == x::(rev_int xs)) =
+  match xs with
+  | [] -> ()
+  | x'::xs' -> (
+    rev_aux xs' x;
+
+    assert(rev_int (snoc xs x) == rev_int (x'::snoc xs' x));
+    assert(rev_int (x'::snoc xs' x) == snoc (rev_int (snoc xs' x)) x');
+    assert(snoc (rev_int (snoc xs' x)) x' == snoc (x::(rev_int xs')) x'); //HI
+    assert(snoc (x::(rev_int xs')) x' == x::(snoc (rev_int xs') x'));
+    assert(x::(snoc (rev_int xs') x') == x::rev_int (x'::xs'))
+  )
+
+let rec rev_rev (xs : list int)
   : Lemma (rev_int (rev_int xs) == xs)
-= admit()
+=
+  match xs with
+  | [] -> ()
+  | x::[] -> ()
+  | x::xs' -> (
+    rev_rev xs';
+    rev_aux (rev_int xs') x
+  )
 
 let rev_injective (xs ys : list int)
   : Lemma (requires rev_int xs == rev_int ys) (ensures xs == ys)
-= admit()
+=
+  assert(rev_int xs == rev_int ys);
+  assert(rev_int (rev_int xs) == rev_int (rev_int ys));
+  rev_rev xs;
+  rev_rev ys
